

5

Use hint and  $-u''(t) = f(t)$ , we have for all  $x_j$ ,  $j=1, \dots, n-1$

$$T_h(x_j) = f(x_j) - \frac{1}{h^2} \left[ \int_{x_j-h}^{x_j} (-f(t))(x_j-h-t)^2 dt - \int_{x_j}^{x_j+h} (-f(t))(x_j+h-t)^2 dt \right]$$

$$:= A_j + B_j + C_j$$

$$A_j = f(x_j), \quad B_j = -\frac{1}{h^2} \int_{x_j-h}^{x_j} f(t)(x_j-h-t)^2 dt, \quad C_j = \frac{1}{h^2} \int_{x_j}^{x_j+h} f(t)(x_j+h-t)^2 dt$$

We note that if  $a, b, c \in \mathbb{R}$ , then  $(a+b+c)^2 \leq 3(a^2+b^2+c^2)$

$$\text{Hence } (T_h(x_j))^2 \leq 3(A_j^2 + B_j^2 + C_j^2) = 3(f(x_j))^2 + B_j^2 + C_j^2$$

For  $B_j$ :

$$|B_j|^2 = \frac{1}{h^4} \left| \int_{x_j-h}^{x_j} f(t)(x_j-h-t)^2 dt \right|^2 \leq \frac{1}{h^4} \left( \int_{x_j-h}^{x_j} |f(t)|^2 dt \right) \left( \int_{x_j-h}^{x_j} (x_j-h-t)^4 dt \right)$$

Use  $s = x_j - t$ , we have

$$\int_{x_j-h}^{x_j} (x_j-h-t)^4 dt = \int_h^0 (s-h)^4 (-ds) = \int_0^h (s-h)^4 ds = \frac{h^5}{5}$$

$$\text{Hence } |B_j|^2 \leq \frac{1}{h^4} \left( \int_{x_j-h}^{x_j} |f(t)|^2 dt \right) \cdot \frac{h^5}{5} = \frac{h}{5} \int_{x_j-h}^{x_j} |f(t)|^2 dt$$

For  $C_j$ , we also use  $s = x_j - t$ , we get

$$\int_{x_j}^{x_j+h} (x_j+h-t)^4 dt = \int_0^h (s+h)^4 (-ds) = \int_{-h}^0 (s+h)^4 ds = \frac{h^5}{5}$$

$$\text{Hence } |C_j|^2 \leq \frac{h}{5} \int_{x_j}^{x_j+h} |f(t)|^2 dt$$

$$\text{So } (T_h(x_j))^2 \leq 3 \left[ (f(x_j))^2 + \frac{h}{5} \int_{x_j-h}^{x_j} |f(t)|^2 dt + \frac{h}{5} \int_{x_j}^{x_j+h} |f(t)|^2 dt \right]$$

$$\Rightarrow \sum_{j=1}^{n-1} (T_h(x_j))^2 \leq 3 \sum_{j=1}^{n-1} (f(x_j))^2 + \frac{3h}{5} \sum_{j=1}^{n-1} \int_{x_j-h}^{x_j} |f|^2 dt + \frac{3h}{5} \sum_{j=1}^{n-1} \int_{x_j}^{x_j+h} |f|^2 dt$$

$$\left( \text{We note that } \sum_{j=1}^{n-1} \int_{x_j-h}^{x_j} |f|^2 dt + \sum_{j=1}^{n-1} \int_{x_j}^{x_j+h} |f|^2 dt \leq 2 \int_0^1 |f(t)|^2 dt = 2 \|f\|_{L^2(0,1)}^2 \right)$$

$$\Rightarrow \sum_{j=1}^{n-1} (T_h(x_j))^2 \leq 3 \sum_{j=1}^{n-1} (f(x_j))^2 + \frac{6h}{5} \|f\|_{L^2(0,1)}^2$$

$$(xh) \Rightarrow \|T_h\|_h^2 = h \sum_{j=1}^{n-1} (T_h(x_j))^2 \leq 3h \sum_{j=1}^{n-1} (f(x_j))^2 + \frac{6h^2}{5} \|f\|_{L^2(0,1)}^2$$

$$= 3 \|f\|_h^2 + \frac{6h^2}{5} \|f\|_{L^2(0,1)}^2$$

$$\leq 3(\|f\|_h^2 + \|f\|_{L^2}^2) \quad \#$$

7.

$$(T_n g)(x_j) = h \sum_{k=1}^{n-1} G(x_j, x_k) g(x_k) \text{ where } g=1$$

$$\text{and we note that } G^k(x_j) = h G(x_j, x_k) = h \begin{cases} x_k(1-x_j), & k \leq j \\ x_j(1-x_k), & k > j \end{cases}$$

$$\text{Hence } T_n g(x_j) = h \sum_{k=1}^{n-1} G(x_j, x_k) \\ = h \left[ \sum_{k=1}^j x_k(1-x_j) + \sum_{k=j+1}^{n-1} x_j(1-x_k) \right]$$

$$\text{Let } h = \frac{1}{n}, \quad x_k = kh, \quad \sum_{k=1}^j x_k = \sum_{k=1}^j kh = h \frac{j(j+1)}{2}$$

$$\Rightarrow h \sum_{k=1}^j x_k(1-x_j) = h^2 \frac{j(j+1)}{2} (1-jh)$$

$$\sum_{k=j+1}^{n-1} (1-x_k) = \sum_{k=j+1}^{n-1} (1-kh)$$

$$= (n-1-j) - h \sum_{k=j+1}^{n-1} k$$

$$= (n-1-j) - h \left( \frac{n(n-1)}{2} - \frac{j(j+1)}{2} \right)$$

$$\Rightarrow h \sum_{k=j+1}^{n-1} x_j(1-x_k) = jh^2 \left[ (n-1-j) - h \left( \frac{n(n-1)}{2} - \frac{j(j+1)}{2} \right) \right]$$

$$\text{So } T_n g(x_j) = \underbrace{h^2 \frac{j(j+1)}{2} (1-jh)}_{\text{Term 1}} + \underbrace{jh^2 \left[ (n-1-j) - h \left( \frac{n(n-1)}{2} - \frac{j(j+1)}{2} \right) \right]}_{\text{Term 2}} \quad (\text{Use } n = \frac{1}{h}, x_j = jh)$$

$$= x_j h \left[ \left( \frac{1}{h} - 1 - j \right) - \frac{\frac{1}{h} - 1}{2} \right] + \frac{x_j h(j+1)}{2}$$

$$= x_j h \left[ \left( \frac{1}{h} - 1 - j \right) - \frac{1-h}{2h} \right] + \frac{1}{2} x_j^2 + \frac{1}{2} x_j h$$

$$= x_j - x_j h - x_j^2 - \frac{1-h}{2} x_j + \frac{1}{2} x_j^2 + \frac{1}{2} x_j h$$

$$= x_j - \cancel{x_j h} - x_j^2 - \frac{1}{2} x_j + \frac{h}{2} x_j + \frac{1}{2} x_j^2 + \frac{1}{2} x_j h$$

$$= \frac{1}{2} x_j (1 - x_j) \quad \#$$

8.

We notice that  $0 \leq \left( \sqrt{\varepsilon} a - \frac{b}{2\sqrt{\varepsilon}} \right)^2$  for  $\forall \varepsilon > 0 \quad \forall a, b \in \mathbb{R}$

$$= \varepsilon a^2 - ab + \frac{b^2}{4\varepsilon}$$

$$\Rightarrow ab \leq \varepsilon a^2 + \frac{b^2}{4\varepsilon} \quad \#$$

9.

From def,  $\|V_h\|_h^2 = (V_h, V_h)_h = h \sum_{k=0}^n C_k V_k^2$

$$\therefore V_k^2 \leq \|V_h\|_{h,\infty}^2$$

$$\therefore h \sum_{k=0}^n C_k V_k^2 \leq h \left[ \sum_{k=0}^n C_k \right] \|V_h\|_{h,\infty}^2$$

$$\sum_{k=0}^n C_k = \frac{1}{2} + \frac{1}{2} + (n-1) \cdot 1 = n$$

$$\Rightarrow \|V_h\|_h^2 = h \sum_{k=0}^n C_k V_k^2 \leq h \cdot n \cdot \|V_h\|_{h,\infty}^2 \quad (h = \frac{1}{n})$$

$$= \|V_h\|_{h,\infty}^2$$

$$\Rightarrow \|V_h\|_h \leq \|V_h\|_{h,\infty} \quad \#$$



11.

$$\text{Let } v_j = (L_h u)_j = - \frac{u_{j+1} - 2u_j + u_{j-1}}{h^2}$$

$$\text{So } (L_h v)_j = - \frac{v_{j+1} - 2v_j + v_{j-1}}{h^2}$$

$$= - \frac{1}{h^2} \left[ - \frac{u_{j+2} - 2u_{j+1} + u_j}{h^2} + 2 \frac{u_{j+1} - 2u_j + u_{j-1}}{h^2} - \frac{u_j - 2u_{j-1} + u_{j-2}}{h^2} \right]$$

$$= \frac{1}{h^4} [u_{j+2} - 4u_{j+1} + 6u_j - 4u_{j-1} + u_{j-2}]$$

$$= (L_h^2 u)_j$$

$$\text{Here } L_h^2 u \approx -u^{(iv)}(x)_\#$$